ADT signatures, BookStore Pick Implementation.

ADT.v
@@ -1,4 +1,4 @@
-Require Export Common Computation.
+Require Export Common Computation ADTSig.
 Require Import Ensembles.
 
 Generalizable All Variables.
@@ -7,39 +7,6 @@ Set Implicit Arguments.
 Local Open Scope type_scope.
 
 (** * Basic ADT definitions *)
-(** Type of a context *)
-
-(** Type of a mutator method. *)
-Definition mutatorMethodType (Ty dom : Type)
-  := Ty    (* Initial model *)
-     -> dom (* Actual argument*)
-     -> Comp Ty (* Final Model *).
-
-(** Type of an obeserver method. *)
-Definition observerMethodType (Ty dom cod : Type)
-  := Ty    (* Initial model *)
-     -> dom (* Actual argument*)
-     -> Comp cod. (* Return value *)
-
-Record ADTSig :=
-  { MutatorIndex : Type;
-     (** The index set of mutators *)
-
-     ObserverIndex : Type;
-     (** The index set of observers *)
-
-     MutatorDom : MutatorIndex -> Type;
-     (** The representation-independent piece of the
-         domain of mutator methods. **)
-
-    ObserverDom : ObserverIndex -> Type;
-     (** The representation-independent piece of the
-         domain of observer methods. **)
-
-    ObserverCod : ObserverIndex -> Type
-     (** The codomain of observer methods. **)
-
-  }.
 
 (** Interface of an ADT *)
 Record ADT (Sig : ADTSig) :=
@@ -54,7 +21,21 @@ Record ADT (Sig : ADTSig) :=
 
     ObserverMethods :
       forall idx : ObserverIndex Sig,
-        observerMethodType Rep (ObserverDom Sig idx) (ObserverCod Sig idx)
+        observerMethodType Rep (fst (ObserverDomCod Sig idx))
+                           (snd (ObserverDomCod Sig idx))
     (** Observer method implementations *)
 
   }.
+
+(*
+Notation "'observer' id ( dom x ) { bod }" :=
+  (id, fun x : dom => bod ) (at level 60).
+
+Notation "'mutator' id ( dom x ) { bod }" :=
+  (id, fun x : dom => bod ) (at level 60).
+
+Notation "'ADT' 'with' 'sig' Sig { mut1 ; .. ; mutn } { obs1 ; .. ; obsn }" :=
+  (@Build_ADT Sig
+             (fun idx => IdxMap.find idx (IdxAdd mut1 .. (IdxAdd mutn IdxMap.empty) ..))
+             (fun idx => IdxMap.find idx (IdxAdd obs1 .. (IdxAdd obsn IdxMap.empty) ..)))
+            (at level 70) *)
