ADTSig.v
@@ -1,0 +1,65 @@
+Require Export Common Computation.
+
+(** Type of a mutator method. *)
+Definition mutatorMethodType (Ty dom : Type)
+  := Ty    (* Initial model *)
+     -> dom (* Actual argument*)
+     -> Comp Ty (* Final Model *).
+
+(** Type of an obeserver method. *)
+Definition observerMethodType (Ty dom cod : Type)
+  := Ty    (* Initial model *)
+     -> dom (* Actual argument*)
+     -> Comp cod. (* Return value *)
+
+Record ADTSig :=
+  { MutatorIndex : Type;
+     (** The index set of mutators *)
+
+     ObserverIndex : Type;
+     (** The index set of observers *)
+
+     MutatorDom : MutatorIndex -> Type;
+     (** The representation-independent piece of the
+         domain of mutator methods. **)
+
+    ObserverDomCod : ObserverIndex -> (Type * Type)
+     (** The representation-independent piece of the
+         domain and codomain of observer methods. **)
+
+  }.
+
+(* Some notations for ADT Signatures. *)
+
+Require Import List String.
+
+Notation "id : 'rep' ✕ dom → cod" :=
+  (@pair string (@prod Type Type) id%string
+         (@pair Type Type dom cod))
+    (at level 60, format "id  :  'rep'  ✕  dom  →  cod" ).
+
+Notation "id : 'rep' ✕ dom → 'rep'" :=
+  (@pair string Type id%string dom)
+    (at level 60, format "id  :  'rep'  ✕  dom  →  'rep'" ).
+
+Fixpoint mutSigMap (sig : list (string * Type)) (id : string)
+: Type :=
+  match sig with
+    | (id', ty) :: sig' => if string_dec id id' then ty else mutSigMap sig' id
+    | _ => unit
+  end.
+
+Fixpoint obsSigMap (sig : list (string * (Type * Type))) (id : string)
+: (Type * Type) :=
+  match sig  with
+    | (id', ty) :: sig' => if string_dec id id' then ty else obsSigMap sig' id
+    | _ => @pair Type Type unit unit
+  end.
+
+Notation "'ADTsignature' { mut1 , .. , mutn ; obs1 , .. , obsn }" :=
+  {| MutatorIndex := string ;
+     ObserverIndex := string ;
+    MutatorDom := mutSigMap (mut1 :: .. (mutn :: []) ..);
+    ObserverDomCod := obsSigMap (obs1 :: .. (obsn :: []) ..)
+  |} (at level 70,
+     format "'ADTsignature'  { '[v' '//' mut1 , '//' .. , '//' mutn ; '//' obs1 , '//' .. , '//' obsn '//'  ']' }").
